spsStep nearly cont

untimed/SpsStep.thy
@@ -6,38 +6,48 @@ begin
 
 default_sort type
 type_synonym 'm SPS = "'m SPF uspec"
-
+  
 definition spsStep_h::"((channel\<rightharpoonup>'m::message) \<Rightarrow> 'm SPS)\<rightarrow> ((channel\<rightharpoonup>'m::message) \<Rightarrow> 'm SPF) set rev"where
-"spsStep_h= (\<Lambda> h. (Rev {(\<lambda>e. if e = x then spf else ufLeast (ufDom\<cdot> spf) (ufDom\<cdot> spf)) | spf x. spf \<in> (Rep_rev_uspec (h x))}))"
+"spsStep_h= (\<Lambda> h. setify\<cdot>(\<lambda>e. fst(Rep_uspec(h e))))"
 
-lemma spsStep_h_mono[simp]:"monofun (\<lambda> h. Rev {(\<lambda>e::(channel\<rightharpoonup>'m::message). if e = z then spf else ufLeast (ufDom\<cdot> spf) (ufDom\<cdot> spf)) |(spf::'m SPF) z. spf \<in> (Rep_rev_uspec (h z))})"
+lemma spsStep_h_mono[simp]:"monofun (\<lambda> h::((channel\<rightharpoonup>'m::message) \<Rightarrow> 'm SPS). setify\<cdot>(\<lambda>e. fst(Rep_uspec(h e))))"
 proof(rule monofunI)
-  fix x y::"(channel \<Rightarrow> 'm option) \<Rightarrow> 'm SPS"
+  fix x y::"(channel \<Rightarrow> 'm::message option) \<Rightarrow> 'm SPS"
   assume a1:"x \<sqsubseteq> y"
-  have "\<And>z. Rep_rev_uspec (y z) \<subseteq> Rep_rev_uspec (x z)"
-    by (metis less_set_def rep_uspec_belowI a1 fun_belowD inv_rev_rep_upsec_below)
-  then have "\<And>z spf. spf \<in> Rep_rev_uspec (y z) \<Longrightarrow> spf \<in> Rep_rev_uspec (x z)"
-    by blast
-  then have "{\<lambda>e. if e = z then spf else ufLeast (ufDom\<cdot>spf) (ufDom\<cdot>spf) |spf z. spf \<in> Rep_rev_uspec (y z)} \<subseteq>
-             {\<lambda>e. if e = z then spf else ufLeast (ufDom\<cdot>spf) (ufDom\<cdot>spf) |spf z. spf \<in> Rep_rev_uspec (x z)}"
-    by blast
-  then show "Rev {\<lambda>e. if e = z then spf else ufLeast (ufDom\<cdot>spf) (ufDom\<cdot>spf) |spf z. spf \<in> Rep_rev_uspec (x z)} \<sqsubseteq>
-       Rev {\<lambda>e. if e = z then spf else ufLeast (ufDom\<cdot>spf) (ufDom\<cdot>spf) |spf z. spf \<in> Rep_rev_uspec (y z)}"
-    by(simp add: less_set_def)
+  then show "setify\<cdot>(\<lambda>e. fst (Rep_uspec (x e))) \<sqsubseteq> setify\<cdot>(\<lambda>e. fst (Rep_uspec (y e)))"
+    by (simp add: below_fun_def fst_monofun monofun_cfun_arg rep_uspec_belowI)
+qed
+   
+lemma spsStep_h_cont[simp]:"cont (\<lambda> h::((channel\<rightharpoonup>'m::message) \<Rightarrow> 'm SPS). setify\<cdot>(\<lambda>e. fst(Rep_uspec(h e))))"
+proof(rule Cont.contI2,simp)
+  fix Y::"nat \<Rightarrow> (channel \<Rightarrow> 'm::message option) \<Rightarrow> 'm SPS"
+  assume a1:"chain Y"
+  assume a2:"chain (\<lambda>i::nat. setify\<cdot>(\<lambda>e. fst (Rep_uspec (Y i e))))"
+  have a3:"\<forall>e. (\<Squnion>i. Y i) e = (\<Squnion>i. Y i e)"
+    by (simp add: a1 lub_fun)
+  have a4:"\<forall>e. (Rep_uspec (\<Squnion>i. Y i e)) = (\<Squnion>i. (Rep_uspec ( Y i e)))"
+    by (metis a1 ch2ch_fun cont2contlubE uspec_rep_cont)
+  have a5:"\<forall>e. fst (\<Squnion>i. (Rep_uspec ( Y i e))) = (\<Squnion>i. fst (Rep_uspec ( Y i e)))"
+    by (smt a1 a4 ch2ch_fun contlub_cfun_arg lub_eq uspecrevset_insert)
+  have a6:" (\<lambda>e. (\<Squnion>i. fst (Rep_uspec ( Y i e)))) = (\<Squnion>i. (\<lambda>e. fst (Rep_uspec ( Y i e))))"
+    apply(subst lub_fun, auto)
+    by (metis (mono_tags, lifting) a1 fst_monofun fun_below_iff po_class.chain_def rep_uspec_belowI)
+  show "setify\<cdot>(\<lambda>e. fst (Rep_uspec ((\<Squnion>i. Y i) e))) \<sqsubseteq> (\<Squnion>i. setify\<cdot>(\<lambda>e. fst (Rep_uspec (Y i e))))"
+    apply(simp add: a1 lub_fun a2 a4 a5 a6)
+    apply(subst contlub_cfun_arg)
+    apply (metis (mono_tags, lifting) a1 below_fun_def fst_monofun po_class.chain_def rep_uspec_belowI)
+    by simp
 qed
   
-      
-lemma spsStep_h_cont[simp]:"cont (\<lambda> h. (Rev {(\<lambda>e::(channel\<rightharpoonup>'m::message). if e = x then spf else ufLeast (ufDom\<cdot> spf) (ufDom\<cdot> spf)) | (spf::'m SPF) x. spf \<in> (Rep_rev_uspec (h x))}))"
-  sorry
 
-lemma spsStep_h_insert:"spsStep_h\<cdot> f = (Rev {(\<lambda>e. if e = x then spf else ufLeast (ufDom\<cdot> spf) (ufDom\<cdot> spf)) | spf x. spf \<in> (Rep_rev_uspec (f x))})"
+lemma spsStep_h_insert:"spsStep_h\<cdot>f = setify\<cdot>(\<lambda>e. fst(Rep_uspec(f e)))"
   by(simp add: spsStep_h_def)
     
 (* like spfStep, copy & pasteonly on SPS *)
-fun spsStep :: "channel set discr \<Rightarrow> channel set discr \<Rightarrow> ((channel\<rightharpoonup>'m::message) \<Rightarrow> 'm SPS) \<rightarrow> 'm SPS" where
-"spsStep (Discr In) (Discr Out) = (\<Lambda> h. Abs_rev_uspec {spfStep In Out\<cdot>g | g. g \<in> inv Rev (spsStep_h\<cdot>h)})"
+fun spsStep :: "channel set \<Rightarrow> channel set \<Rightarrow> ((channel\<rightharpoonup>'m::message) \<Rightarrow> 'm SPS) \<rightarrow> 'm SPS" where
+"spsStep In Out = (\<Lambda> h. Abs_rev_uspec {spfStep In Out\<cdot>g | g. g \<in> inv Rev (spsStep_h\<cdot>h)} In Out)"
 
-lemma spsStep_mono[simp]:"monofun (\<lambda>h::(channel \<Rightarrow> 'a::message option) \<Rightarrow> ('a stream\<^sup>\<Omega>) ufun uspec. Abs_rev_uspec {spfStep In Out\<cdot>g |g::(channel \<Rightarrow> 'a option) \<Rightarrow> ('a stream\<^sup>\<Omega>) ufun. g \<in> inv Rev (spsStep_h\<cdot>h)})"
+lemma spsStep_mono[simp]:"monofun (\<lambda>h::(channel \<Rightarrow> 'a::message option) \<Rightarrow> ('a stream\<^sup>\<Omega>) ufun uspec. Abs_rev_uspec {spfStep In Out\<cdot>g |g::(channel \<Rightarrow> 'a option) \<Rightarrow> ('a stream\<^sup>\<Omega>) ufun. g \<in> inv Rev (spsStep_h\<cdot>h)} In Out)"
 proof(rule monofunI)
   fix x y::"(channel \<Rightarrow> 'm::message option) \<Rightarrow> 'm SPS" 
   assume a1: "x \<sqsubseteq> y"
@@ -55,29 +65,48 @@ proof(rule monofunI)
     by (simp add: ufclRan_ufun_def)
   have h4:"\<And>f h. f\<in>{spfStep In Out\<cdot>g |g::(channel \<Rightarrow> 'm option) \<Rightarrow> ('m stream\<^sup>\<Omega>) ufun. g \<in> inv Rev (spsStep_h\<cdot>h)} \<Longrightarrow> \<exists>g. f = spfStep In Out\<cdot>g"
     by auto
-  have h2:"uspecWell {spfStep In Out\<cdot>g |g::(channel \<Rightarrow> 'm option) \<Rightarrow> ('m stream\<^sup>\<Omega>) ufun. g \<in> inv Rev (spsStep_h\<cdot>x)}"
-    apply(simp add: uspecWell_def)
-    apply(rule_tac x="In" in exI)
-    apply(rule_tac x="Out" in exI)
+  have h2:"uspecWell (Rev {spfStep In Out\<cdot>g |g::(channel \<Rightarrow> 'm option) \<Rightarrow> ('m stream\<^sup>\<Omega>) ufun. g \<in> inv Rev (spsStep_h\<cdot>x)}) (Discr In) (Discr Out)"
     using h2 h3 by auto
-  have h3:"uspecWell {spfStep In Out\<cdot>g |g::(channel \<Rightarrow> 'm option) \<Rightarrow> ('m stream\<^sup>\<Omega>) ufun. g \<in> inv Rev (spsStep_h\<cdot>y)}"
-    apply(simp add: uspecWell_def)
-    apply(rule_tac x="In" in exI)
-    apply(rule_tac x="Out" in exI)
-    by (metis finite h3 spfstep_dom ufclDom_ufun_def)
-  show "Abs_rev_uspec {spfStep In Out\<cdot>g |g. g \<in> inv Rev (spsStep_h\<cdot>x)} \<sqsubseteq>
-       Abs_rev_uspec {spfStep In Out\<cdot>g |g. g \<in> inv Rev (spsStep_h\<cdot>y)}"
-    by (metis (mono_tags, lifting) h1 h2 h3 rep_abs_rev_simp uspec_belowI)
+  have h3:"uspecWell (Rev {spfStep In Out\<cdot>g |g::(channel \<Rightarrow> 'm option) \<Rightarrow> ('m stream\<^sup>\<Omega>) ufun. g \<in> inv Rev (spsStep_h\<cdot>y)}) (Discr In) (Discr Out)"
+    by (metis (no_types, lifting) SetPcpo.less_set_def h1 h2 subsetCE uspecWell.simps)
+  show "Abs_rev_uspec {spfStep In Out\<cdot>g |g. g \<in> inv Rev (spsStep_h\<cdot>x)} In  Out\<sqsubseteq>
+       Abs_rev_uspec {spfStep In Out\<cdot>g |g. g \<in> inv Rev (spsStep_h\<cdot>y)} In Out"
+    by (metis (no_types, lifting) Pair_below_iff below_refl below_rev.simps below_uspec_def h1 h2 h3 rep_abs_uspec)
 qed
   
-lemma spsStep_cont[simp]:"cont (\<lambda>h. Abs_rev_uspec {spfStep In Out\<cdot>g | g. g \<in>inv Rev (spsStep_h\<cdot>h)})"
+lemma spsStep_cont[simp]:assumes "finite In" shows"cont (\<lambda>h. Abs_rev_uspec {spfStep In Out\<cdot>g | g. g \<in>inv Rev (spsStep_h\<cdot>h)} In Out)"
 proof(rule Cont.contI2, simp)
-  fix Y::"nat \<Rightarrow> ((channel \<Rightarrow> 'm::message option) \<Rightarrow> 'm SPS)"
+  fix Y::"nat \<Rightarrow> ((channel \<Rightarrow> 'a option) \<Rightarrow> 'a SPS)"
   assume a1:"chain Y"
-  assume a2:"chain (\<lambda>i::nat. Abs_rev_uspec {spfStep In Out\<cdot>g |g. g \<in> inv Rev (spsStep_h\<cdot>(Y i))})"
-  show "Abs_rev_uspec {spfStep In Out\<cdot>g |g. g \<in> inv Rev (spsStep_h\<cdot>(\<Squnion>i::nat. Y i))} \<sqsubseteq>
-       (\<Squnion>i::nat. Abs_rev_uspec {spfStep In Out\<cdot>g |g. g \<in> inv Rev (spsStep_h\<cdot>(Y i))})"
-  apply(simp add: a1 contlub_cfun_fun contlub_cfun_arg)
+  assume a2:"chain (\<lambda>i. Abs_rev_uspec {spfStep In Out\<cdot>g |g. g \<in> inv Rev (spsStep_h\<cdot>(Y i))} In Out)"
+  have h1:"\<forall>i. uspecWell (Rev {spfStep In Out\<cdot>g |g. g \<in> inv Rev (spsStep_h\<cdot>(Y i))}) (Discr In) (Discr Out)"
+    by (smt finite mem_Collect_eq spfstep_dom spfstep_ran ufclDom_ufun_def ufclRan_ufun_def uspecWell.simps)
+  have h2:"uspecWell (Rev {spfStep In Out\<cdot>g |g::(channel \<Rightarrow> 'a option) \<Rightarrow> ('a stream\<^sup>\<Omega>) ufun. g \<in> inv Rev (\<Squnion>i::nat. spsStep_h\<cdot>(Y i))}) (Discr In) (Discr Out)"
+    by (smt finite mem_Collect_eq spfstep_dom spfstep_ran ufclDom_ufun_def ufclRan_ufun_def uspecWell.simps)
+  have h3:"Rep_uspec (Abs_uspec (\<Squnion>i::nat. (Rev {spfStep In Out\<cdot>g |g::(channel \<Rightarrow> 'a option) \<Rightarrow> ('a stream\<^sup>\<Omega>) ufun. g \<in> inv Rev (spsStep_h\<cdot>(Y i))}, Discr In, Discr Out)))
+        =  (\<Squnion>i::nat. (Rev {spfStep In Out\<cdot>g |g::(channel \<Rightarrow> 'a option) \<Rightarrow> ('a stream\<^sup>\<Omega>) ufun. g \<in> inv Rev (spsStep_h\<cdot>(Y i))}, Discr In, Discr Out))"
+    by (metis (mono_tags, lifting) a2 cont2contlubE h1 lub_eq lub_uspec rep_abs_uspec uspec_rep_cont)
+  have h4:"chain (\<lambda>i::nat. Rev {g. \<forall>m. g m \<in> Rep_rev_uspec (Y i m)})"
+    by (smt Collect_mono SetPcpo.less_set_def a1 below_fun_def below_rev.elims(2) below_rev.simps fst_monofun inv_rev_rev po_class.chain_def rep_uspec_belowI subsetCE) 
+  have h5:"(\<Squnion>i. (Rev {spfStep In Out\<cdot>g |g. \<forall>m. g m \<in> Rep_rev_uspec (Y i m)}, Discr In, Discr Out)) = ((\<Squnion>i. Rev{spfStep In Out\<cdot>g |g. \<forall>m. g m \<in> Rep_rev_uspec (Y i m)}), Discr In, Discr Out )"
+    sorry
+  have h6:"chain (\<lambda>i::nat. Rev {spfStep In Out\<cdot>g |g::(channel \<Rightarrow> 'a option) \<Rightarrow> ('a stream\<^sup>\<Omega>) ufun. \<forall>m::channel \<Rightarrow> 'a option. g m \<in> Rep_rev_uspec (Y i m)})"
+    by (smt Collect_mono SetPcpo.less_set_def a1 below_rev.elims(2) below_rev.simps fst_monofun fun_below_iff inv_rev_rev po_class.chain_def rep_uspec_belowI subsetCE)
+  show "Abs_rev_uspec {spfStep In Out\<cdot>g |g. g \<in> inv Rev (spsStep_h\<cdot>(\<Squnion>i. Y i))} In Out \<sqsubseteq>
+       (\<Squnion>i. Abs_rev_uspec {spfStep In Out\<cdot>g |g. g \<in> inv Rev (spsStep_h\<cdot>(Y i))} In Out)"
+    apply(simp add: a1 contlub_cfun_fun contlub_cfun_arg)
+    apply(simp add: below_uspec_def)
+    apply(simp only: h2 rep_abs_uspec)
+    apply(simp add: lub_uspec a2)
+    apply(simp only: h1 rep_abs_uspec h3)
+    apply(simp add: a1 spsStep_h_insert)
+    apply(simp add: setify_def inv_rev_rev h5)
+    apply(subst setrevLubEqInterII, simp add: h4)
+    apply(subst setrevLubEqInter, simp add: h6 ,simp add:inv_rev_rev rev_inv_rev)
+    apply(simp add: less_set_def)
+    apply(simp add: assms spfstep_insert)
+    apply auto 
+    apply(simp add: assms spfstep_insert)
     sorry
 qed
   
